more tactics

Lean2055/Basic.lean
@@ -61,6 +61,12 @@ instance (U : Type _) : SDiff (Set U) := ⟨fun A B x => x ∈ A ∧ x ∉ B⟩
 
 instance (U : Type _) : EmptyCollection (Set U) := ⟨fun _ => False⟩
 
+instance (U : Type _) : Singleton U (Set U) where
+  singleton x y := y = x
+
+instance (U : Type _) : Insert U (Set U) where
+  insert a A x := x = a ∨ x ∈ A
+
 protected theorem Subset.def {U : Type _} (A B : Set U) : A ⊆ B ↔ ∀ (x : U), x ∈ A → x ∈ B := .rfl
 
 protected theorem Inter.def {U : Type _} (A B : Set U) (x : U) : x ∈ A ∩ B ↔ x ∈ A ∧ x ∈ B := .rfl
@@ -71,9 +77,104 @@ protected theorem SDiff.def {U : Type _} (A B : Set U) (x : U) : x ∈ A \ B ↔
 
 protected theorem Empty.def {U : Type _} (x : U) : x ∈ (∅ : Set U) ↔ False := .rfl
 
+protected theorem Empty.forall {U : Type _} (P : U → Prop) : (∀ x, x ∈ (∅ : Set U) → P x) ↔ True := by
+  simp [Empty.def]
+
+protected theorem Empty.exists {U : Type _} (P : U → Prop) : (∃ x, x ∈ (∅ : Set U) ∧ P x) ↔ False := by
+  simp [Empty.def]
+
+protected theorem Singleton.def {U : Type _} (a x : U) : x ∈ (singleton a : Set U) ↔ x = a := .rfl
+
+protected theorem Singleton.forall {U : Type _} (a : U) (P : U → Prop) :
+    (∀ x, x ∈ (singleton a : Set U) → P x) ↔ P a := by
+  constructor
+  · intro h; exact h a rfl
+  · intro | h, _, rfl => exact h
+
+protected theorem Singleton.exists {U : Type _} (a : U) (P : U → Prop) :
+    (∃ x, x ∈ (singleton a : Set U) ∧ P x) ↔ P a := by
+  constructor
+  · intro | ⟨_, rfl, h⟩ => exact h
+  · intro h; exists a
+
+protected theorem Insert.def {U : Type _} (A : Set U) (a x : U) : x ∈ insert a A ↔ x = a ∨ x ∈ A := .rfl
+
+protected theorem Insert.forall {U : Type _} (A : Set U) (a : U) (P : U → Prop) :
+    (∀ x, x ∈ insert a A → P x) ↔ P a ∧ (∀ x, x ∈ A → P x) := by
+  constructor
+  · intro h
+    constructor
+    · apply h
+      simp [insert]
+      left
+      rfl
+    · intro x hx
+      apply h
+      simp [insert]
+      right
+      exact hx
+  · intro ⟨ha, h⟩ x hx
+    simp [insert] at hx
+    match hx with
+    | .inl rfl => exact ha
+    | .inr hx => apply h; exact hx
+
+protected theorem Insert.exists {U : Type _} (A : Set U) (a : U) (P : U → Prop) :
+    (∃ x, x ∈ insert a A ∧ P x) ↔ P a ∨ (∃ x, x ∈ A ∧ P x) := by
+  constructor
+  · intro ⟨x, hx, h⟩
+    match hx with
+    | .inl rfl => left; exact h
+    | .inr hx => right; exists x
+  · intro h
+    match h with
+    | .inl ha =>
+      exists a
+      constructor
+      · left; rfl
+      · exact ha
+    | .inr ⟨x, hx, h⟩ =>
+      exists x
+      constructor
+      · right; exact hx
+      · exact h
+
+def setOf {U : Type _} (P : U → Prop) : Set U := P
+
+protected theorem SetOf.def {U : Type} (P : U → Prop) (x : U) : x ∈ setOf P ↔ P x := .rfl
+
+def Dom {U V : Type _} (R : Set (U × V)) : Set U := setOf fun x : U => ∃ (y : V), (x, y) ∈ R
+
+def Ran {U V : Type _} (R : Set (U × V)) : Set V := setOf fun y : V => ∃ (x : U), (x, y) ∈ R
+
 macro_rules
 | `(tactic| unfold Subset $[$loc:location]?) => `(tactic| simp only [Subset.def] $[$loc]?)
 | `(tactic| unfold Inter $[$loc:location]?) => `(tactic| simp only [Inter.def] $[$loc]?)
 | `(tactic| unfold Union $[$loc:location]?) => `(tactic| simp only [Union.def] $[$loc]?)
 | `(tactic| unfold SDiff $[$loc:location]?) => `(tactic| simp only [SDiff.def] $[$loc]?)
 | `(tactic| unfold Empty $[$loc:location]?) => `(tactic| simp only [Empty.def] $[$loc]?)
+| `(tactic| unfold SetOf $[$loc:location]?) => `(tactic| simp only [SetOf.def] $[$loc]?)
+| `(tactic| unfold Enum $[$loc:location]?) =>
+  `(tactic|
+      (try simp only [Insert.forall, Insert.exists,
+        Singleton.forall, Singleton.exists,
+        Empty.forall, Empty.exists, -eq_self] $[$loc]?) <;>
+      (try simp only [Insert.def, Singleton.def, Empty.def, -eq_self] $[$loc]?))
+
+syntax (name := setBuilder) "{" Batteries.ExtendedBinder.extBinder " | " term "}" : term
+
+@[term_elab setBuilder]
+def elabSetBuilder : Lean.Elab.Term.TermElab
+  | `({ $x:ident | $p }), expectedType? => do
+    Lean.Elab.Term.elabTerm (← `(setOf fun $x:ident ↦ $p)) expectedType?
+  | `({ $x:ident : $t | $p }), expectedType? => do
+    Lean.Elab.Term.elabTerm (← `(setOf fun $x:ident : $t ↦ $p)) expectedType?
+  | `({ $x:ident $b:binderPred | $p }), expectedType? => do
+    Lean.Elab.Term.elabTerm (← `(setOf fun $x:ident ↦ satisfies_binder_pred% $x $b ∧ $p)) expectedType?
+  | _, _ => Lean.Elab.throwUnsupportedSyntax
+
+@[app_unexpander setOf]
+def setOf.unexpander : Lean.PrettyPrinter.Unexpander
+  | `($_ fun $x:ident ↦ $p) => `({ $x:ident | $p })
+  | `($_ fun ($x:ident : $ty:term) ↦ $p) => `({ $x:ident : $ty:term | $p })
+  | _ => throw ()
